CollapsingTowers/TwoLevelRec/SyntacticTyping/Defs.lean
@@ -3,3 +3,4 @@ import CollapsingTowers.TwoLevelRec.SyntacticTyping.Weakening
 import CollapsingTowers.TwoLevelRec.SyntacticTyping.Shrinking
 import CollapsingTowers.TwoLevelRec.SyntacticTyping.PresvSubst
 import CollapsingTowers.TwoLevelRec.SyntacticTyping.PresvMaping
+import CollapsingTowers.TwoLevelRec.SyntacticTyping.PresvHead
