CollapsingTowers/TwoLevelRec/SyntacticTyping/PresvHead.lean
@@ -1,0 +1,164 @@
+import CollapsingTowers.TwoLevelRec.Semantic.Defs
+import CollapsingTowers.TwoLevelRec.SyntacticTyping.PresvSubst
+import CollapsingTowers.TwoLevelRec.SyntacticTyping.PresvMaping
+import CollapsingTowers.TwoLevelRec.SyntacticTyping.Shrinking
+
+lemma typing.escape_strengthened :
+  ∀ Γ e τ,
+    typing Γ 𝟚 e τ ∅ →
+    typing (escape Γ) 𝟙 e τ ∅ :=
+  by
+  generalize HEq𝕊 : 𝟚 = 𝕊
+  intros Γ e τ Hτ
+  apply
+    @typing.rec
+      (fun Γ 𝕊 e τ φ (H : typing Γ 𝕊 e τ φ) =>
+          𝟚 = 𝕊 →
+          typing (escape Γ) 𝟙 e τ φ)
+      (fun Γ e τ φ (H : typing_reification Γ e τ φ) => true)
+  <;> (intros; try contradiction)
+  case fvar x _ Hbinds Hwbt HEq𝕊 =>
+    apply typing.fvar
+    apply binds.escape; apply Hbinds
+    apply wbt.escape; apply Hwbt
+  case fix Hwbt Hclose IH HEq𝕊 =>
+    rw [← HEq𝕊, escape] at IH
+    apply typing.fix; rw [← escape.length]
+    apply IH; rfl
+    apply wbt.escape; apply Hwbt
+    rw [← escape.length]; apply Hclose
+  case app₁ IHf IHarg HEq𝕊 =>
+    apply typing.app₁
+    apply IHf; apply HEq𝕊
+    apply IHarg; apply HEq𝕊
+  case lit => apply typing.lit
+  case lets Hwbt Hclose IHb IHe HEq𝕊 =>
+    rw [← HEq𝕊, escape] at IHe
+    apply typing.lets
+    apply IHb; apply HEq𝕊
+    rw [← escape.length]; apply IHe; rfl
+    apply wbt.escape; apply Hwbt
+    rw [← escape.length]; apply Hclose
+  case pure => simp
+  case reify => simp
+  apply Hτ; apply HEq𝕊
+
+lemma typing.escape :
+  ∀ Γ e τ,
+    closed e →
+    typing Γ 𝟚 e τ ∅ →
+    typing Γ 𝟙 e τ ∅ :=
+  by
+  intros Γ e τ Hclose Hτ
+  rw [← List.append_nil Γ]; apply typing.weakening
+  rw [escape.nil]; apply typing.escape_strengthened
+  induction Γ with
+  | nil => apply Hτ
+  | cons _ _ IH =>
+    apply IH
+    apply typing.shrinking; apply Hτ
+    apply closed.inc; apply Hclose; omega
+
+theorem preservation.head :
+  ∀ Γ e₀ e₁ τ φ,
+    head e₀ e₁ →
+    lc e₀ →
+    typing Γ 𝟙 e₀ τ φ →
+    typing Γ 𝟙 e₁ τ φ :=
+  by
+  intros Γ e₀ e₁ τ φ Hhead Hlc Hτ
+  cases Hhead
+  case lets Hvalue =>
+    cases Hτ
+    case lets e v τ φ _ _ Hτv Hclose Hτe =>
+      have Hpure : φ = (∅ : Effect) := by cases Hvalue <;> cases Hτv <;> rfl
+      rw [Hpure] at Hτv; simp [Hpure]
+      rw [← intros.subst]; apply preservation.subst
+      apply Hτv; apply Hτe; apply Hclose
+  case app₁ Hvalue =>
+    cases Hτ
+    case app₁ φ Hτv Hτf =>
+      cases Hτf
+      case fix Hclose _ Hτe =>
+        have Hpure : φ = (∅ : Effect) := by cases Hvalue <;> cases Hτv <;> rfl
+        rw [Hpure] at Hτv; simp [Hpure]
+        admit
+  case app₂ =>
+    cases Hτ
+    case app₂ Hτ₀ Hτ₁ =>
+      cases Hτ₀
+      case code_fragment Hwbt₀ Hbinds₀ =>
+        cases Hτ₁
+        case code_fragment Hwbt₁ Hbinds₁ =>
+          apply typing.reflect
+          rw [← union_pure_right ∅, ← union_pure_right (∅ ∪ ∅)]
+          apply typing.app₁
+          apply typing.fvar; apply Hbinds₀; apply Hwbt₀
+          apply typing.fvar; apply Hbinds₁; apply Hwbt₁
+  case lift_lit =>
+    cases Hτ
+    case lift_lit Hτ =>
+      apply typing.reflect
+      apply typing.lit
+    case lift_fix => contradiction
+  case lift_fix e =>
+    cases Hτ
+    case lift_fix Hτ =>
+      cases Hτ
+      case fix Hclose Hwbt Hτe =>
+        rw [← intros.maping𝕔 Γ.length]
+        all_goals admit
+    case lift_lit => contradiction
+  case fix𝕔 e =>
+    cases Hτ
+    case fix𝕔 Hwbt Hτ Hclose =>
+      apply typing.reflect
+      apply typing.fix
+      cases Hτ with
+      | pure _ _ _ Hτ =>
+        generalize Eqe : ({0 ↦ Γ.length + 1}{1 ↦ Γ.length} e) = E
+        simp [Eqe] at Hτ
+        cases Hτ with
+        | code_rep _ _ _ Hτ => apply Hτ
+      | reify _ _ _ _ Hτ =>
+        generalize Eqe : ({0 ↦ Γ.length + 1}{1 ↦ Γ.length} e) = E
+        simp [Eqe] at Hτ
+        cases Hτ with
+        | code_fragment _ _ _ Hbinds Hwbt =>
+          apply typing.fvar
+          apply Hbinds; apply Hwbt
+      apply Hwbt
+      apply Hclose
+  case lets𝕔 e =>
+    cases Hτ
+    case lets𝕔 Hwbt Hτb Hτe Hclose =>
+      apply typing.code_rep
+      rw [← union_pure_right ∅]
+      apply typing.lets
+      apply Hτb
+      cases Hτe with
+      | pure _ _ _ Hτ =>
+        generalize Eqe : ({0 ↦ Γ.length} e) = E
+        simp [Eqe] at Hτ
+        cases Hτ with
+        | code_rep _ _ _ Hτ => apply Hτ
+      | reify _ _ _ _ Hτ =>
+        generalize Eqe : ({0 ↦ Γ.length} e) = E
+        simp [Eqe] at Hτ
+        cases Hτ with
+        | code_fragment _ _ _ Hbinds Hwbt =>
+          apply typing.fvar
+          apply Hbinds; apply Hwbt
+      apply Hwbt
+      apply Hclose
+  case run =>
+    cases Hτ
+    case run Hclose Hτ =>
+      cases Hτ with
+      | pure _ _ _ Hτ =>
+        cases Hτ
+        case code_rep Hτ =>
+          apply typing.escape
+          apply Hclose; apply Hτ
+      | reify _ _ _ _ Hτ =>
+        cases Hτ; contradiction
